\begin{enumerate}[(a)]
\item $\frac{V_{out}(s)}{V_{in}(s)}  = \frac{1}{0.125s^2 + 0.5s +1}$
\item For $v_{in}(t) = 1$, $V_{in}(s) = \frac{1}{s}$. 
\begin{align*}
V_{out}(s) & = \frac{1}{0.125s^2 + 0.5s + 1}\frac{1}{s} \\
& = \frac{8}{(s^{2}+4s+8)s} = \frac{A}{s} + \frac{Bs+C}{s^{2}+4s+8}
\end{align*}
Using residue theorem,
\[
A = \left.  \frac{8}{(s^{2}+4s+8)} \right|_{s=0} = 1
\]
Putting right hand side over common denominator,
\[
\frac{8}{(s^{2}+4s+8)s} = \frac{s^{2}+4s+8+Bs^2+Cs}{(s^{2}+4s+8)s}. 
\]
Equating coefficients,
\begin{align*}
s^{2}:\quad 0 &= 1+B\\
s:\quad 0 &= 4+C 
\end{align*}
Thus, $B =-1$, $C=-4$. By completing the square, the denominator $s^{2}+4s+8$ can be written as $(s+2)^2 + 4 $
\begin{align*}
\frac{8}{(s^{2}+4s+8)s} &= \frac{1}{s} + \frac{-(s+4)}{(s+2)^2+4}\\
&= \frac{1}{s} + \frac{-(s+2)}{(s+2)^2+4} + \frac{-2}{(s+2)^2 + 4}
\end{align*}
Using a Laplace Transform table,
\[
v_{out}(t) = 1 - e^{-2t}\cos(2t) - e^{-2t}\sin(2t) \quad t\geq 0
\]
\item 
\begin{alltt}
t=simout.Time;
v_out = 1 -exp(-2*t).*cos(2*t) - exp(-2*t).*sin(2*t);
plot(t,simout.Data,\T{}r-\T{},t,v_out,\T{}b--\T{})
legend(\T{}Simulation\T{},\T{}Analytical Solution\T{})
xlabel(\T{}Time (s)\T{})
ylabel(\T{}Voltage (V)\T{})
\end{alltt}
\begin{center}
\includegraphics[width=5in]{\mainfolder/LectureNotes/\lecturefolder/HomeworkProblems/Problem19/SimulationResults}
\end{center}
\end{enumerate}